semantics/proofs_new.v
@@ -1,0 +1,46 @@
+Set Warnings "-notation-overridden,-parsing".
+From Coq Require Import Bool.Bool Init.Nat Arith.Arith Arith.EqNat
+     Init.Datatypes Strings.String Program Logic.FunctionalExtensionality.
+Require Export Coq.Strings.String.
+From mathcomp Require Import ssreflect ssrfun ssrbool eqtype seq fintype ssrnat ssrfun.
+From TLC Require Import LibTactics LibLogic.
+From Semantics Require Export programs semantics algorithms lemmas_1
+     lemmas_0 proofs_0. (*shouldn't have to import both of these*)
+
+Implicit Types N: nvmem. Implicit Types V: vmem.
+Implicit Types O: obseq.
+Implicit Types c: command.
+Implicit Types W: the_write_stuff.
+Implicit Types x: smallvar.
+(*actually ask arthur about that thing with the quantifer
+ as against the implication*)
+
+Definition end_com c := c = Ins skip \/ exists(crem: command)(w: warvars), c= (incheckpoint w);; crem.
+
+Definition nvm_eq N1 N2 := subseq (getdomain N1) (getdomain N2) /\
+                           subseq (getdomain N2) (getdomain N1).
+
+Lemma hacky_nvm_eq N1 N2 : nvm_eq N1 N2 <-> (getdomain N1) = (getdomain N2).
+Admitted.
+
+(*why do you include the volatile memory
+ maybe to make the traces more tractable
+ leave it in for now, can always take it out*)
+Inductive all_diff_in_fw: nvmem -> vmem -> command -> nvmem -> Prop :=
+  Diff_in_FW: forall{N1 V1 c1 N2 V2 c2 N1c O W} (T: trace_c (N1, V1, c1) (N2, V2, c2) O W),
+    end_com c2 -> checkpoint \notin O -> (*c2 is nearest checkpoint or termination*)
+    (getdomain N1) = (getdomain N2) -> (*alternatively
+                                       could check N2 domain as well instead of this*)
+   (forall(el: el_loc), (inr el) \in (getdomain N1) -> ((getmap N1) (inr el)) = ((getmap N2) (inr el))) ->
+( forall(l: loc ), l \in (getdomain N1) -> ((getmap N1) l <> (getmap N2) l) -> (l \in getfstwt W))
+-> all_diff_in_fw N1 V1 c1 N1c.
+
+Lemma two Ni Ni1 V V1 c c1 Nc Nc1 O W: all_diff_in_fw Ni V c Nc ->
+                              cceval_w (Ni, V, c) O (Ni1, V1, c1) W ->
+                              (cceval_w (Nc, V, c) O (Nc1, V1, c1) W /\
+                              forall(l: loc), l \in (getwt W) -> ((getmap Ni1) l = (getmap Nc1) l)).
+Admitted.
+
+Lemma three N0 V0 c0 Ni Ni1 V V1 c c1 Nc Nc1 O W:
+  all_diff_in_fw Ni V c Nc ->
+  trace_i ((N0, V0, c0))
